First attempt of [WF_fv]. It's wrong...

examples/ghc/theories/FV.v
@@ -1,4 +1,78 @@
+Require Import Core.
 Require Import FV.
+Require Import Proofs.ContainerAxioms.
+
+Require Import Coq.Lists.List.
+Require Import Coq.Bool.Bool.
+
+Require Import GHC.Base.
+Import GHC.Base.ManualNotations.
+
+Set Bullet Behavior "Strict Subproofs".
+
+Axiom realUnique_eq : forall x y,
+    (x == y) = (realUnique x == realUnique y).
+
+(** For simplicity, only consider deletion for now. *)
+Definition WF_fv (fv : FV) : Prop :=
+  forall f bs l vs,
+    (forall x, elemVarSet x vs && elemVarSet x bs = false) ->
+    let '(l', vs') := fv f bs (l, vs) in
+    (forall x, elemVarSet x bs = true -> elemVarSet x vs' = false) /\
+    (bs = emptyVarSet -> vs = vs').
+
+Lemma elemVarSet_neq :
+  forall x y vs,
+    elemVarSet x vs = true ->
+    elemVarSet y vs = false ->
+    x == y = false.
+Proof.
+  intros. apply not_true_is_false. intro. revert H. revert H0.
+  unfold elemVarSet, UniqSet.elementOfUniqSet; destruct vs.
+  unfold UniqFM.elemUFM; destruct u. intro H.
+  rewrite member_eq with (k':=(Unique.getWordKey (Unique.getUnique x))) in H.
+  - rewrite H. discriminate.
+  - simpl. rewrite realUnique_eq in H1. cbn in H1.
+    apply Nat.eqb_eq in H1. rewrite H1. cbn. apply N.eqb_refl.
+Qed.
+
+Lemma elemVarSet_extendVarSet :
+  forall x y vs,
+    x == y = false ->
+    elemVarSet x vs = false ->
+    elemVarSet x (extendVarSet vs y) = false.
+Proof.
+  intros. unfold extendVarSet, UniqSet.addOneToUniqSet. revert H0.
+  destruct vs. unfold elemVarSet, UniqSet.elementOfUniqSet.
+  unfold UniqFM.addToUFM, UniqFM.elemUFM. destruct u. intros Hmem.
+  rewrite member_insert. apply orb_false_iff; split; [ | assumption].
+  apply not_true_is_false. intro.
+  cbn in H0. apply N.eqb_eq in H0. apply Nat2N.inj in H0.
+  rewrite <- Nat.eqb_eq, <- realUnique_eq in H0. rewrite H in H0. discriminate.
+Qed.  
+
+Lemma unit_FV_WF :
+  forall x, WF_fv (unitFV x).
+Proof.
+  unfold WF_fv; intros.
+  destruct (unitFV x f bs (l, vs)) eqn:Hfv; intros.
+  unfold unitFV in Hfv.
+  destruct (elemVarSet x bs) eqn:Hin.
+  - inversion Hfv; subst. split; [| reflexivity].
+    intros x0 H'. specialize (H x0).
+    apply andb_false_elim in H; destruct H; [assumption | congruence].
+  - destruct (elemVarSet x vs) eqn:Hin'.
+    + inversion Hfv; subst. split; [| reflexivity].
+      intros. specialize (H x0).
+      apply andb_false_elim in H; destruct H; [assumption | congruence].
+    + destruct (f x) eqn:Hf.
+      * inversion Hfv; subst. split.
+        -- intros. specialize (H x0); apply andb_false_elim in H.
+           destruct H; try congruence.
+           apply (elemVarSet_neq _ _ _ H0) in Hin.
+           apply elemVarSet_extendVarSet; try assumption.
+        -- inversion Hfv; subst; assumption.
+Qed.
 
 Lemma union_empty_l : forall fv, FV.unionFV FV.emptyFV fv = fv.
 Proof. reflexivity. Qed.
